More thoughts on bisimulations, (WIP) prove basic properties of the semantics

src/Concurrent/InductiveNodeSemantics.v
@@ -1,4 +1,5 @@
 From CoreErlang.Concurrent Require Export NodeSemantics.
+From CoreErlang.FrameStack Require Export SubstSemanticsLemmas.
 
 Import ListNotations.
 
@@ -12,6 +13,8 @@ Inductive closureNodeSem : Node -> list (Action * PID) -> Node -> Prop :=
   n -[(a,ι)::l]ₙ->* n''
 where "n -[ l ]ₙ->* n'" := (closureNodeSem n l n').
 
+(* Properties *)
+
 Theorem closureNodeSem_trans :
   forall n n' l, n -[l]ₙ->* n' -> forall n'' l', n' -[l']ₙ->* n''
 ->
@@ -21,5 +24,956 @@ Proof.
   * exact H.
   * eapply n_trans. exact H.
     eapply (IHD1 _ _ H0).
+Qed.
+
+Definition internals (n n' : Node) : Prop :=
+  exists l, Forall (fun e => e.1 = τ) l /\ n -[l]ₙ->* n'.
+
+Notation "n -->* n'" := (internals n n') (at level 50).
+
+Theorem internals_refl :
+  forall n, n -->* n.
+Proof.
+  intros. exists []. split; auto. constructor.
+Qed.
+
+Theorem internals_trans :
+  forall n n' n'', n -->* n' -> n' -->* n''
+->
+  n -->* n''.
+Proof.
+  intros. destruct H as [l1 [All1 D1]]. destruct H0 as [l2 [All2 D2]].
+  exists (l1 ++ l2). split.
+  * now apply Forall_app.
+  * eapply closureNodeSem_trans; eassumption.
+Qed.
+
+Theorem bool_from_lit_val :
+  forall y e, Some y = bool_from_lit e -> VALCLOSED e.
+Proof.
+  destruct e; intros; inversion H.
+  now constructor.
+Qed.
+
+Definition onlyOne (a : Action) (ι : PID) (n n''' : Node) :=
+  exists n' n'', n -->* n' /\ n' -[a|ι]ₙ-> n'' /\ n'' -->* n'''.
+
+Notation "n -[* a | ι *]-> n'" := (onlyOne a ι n n') (at level 60).
+
+Lemma internal_determinism :
+  forall p p' a, p -⌈a⌉-> p' -> forall p'', p -⌈a⌉-> p'' -> p' = p''.
+Proof.
+  intros p p' a IH. induction IH; intros; try now inv H.
+  * inv H0; try (now inv H; cbn in *; invSome).
+    - eapply step_determinism in H. 2: exact H7. destruct H. now subst.
+  * inv H0; firstorder; subst; try congruence.
+  * inv H0; firstorder; subst; try congruence.
+  * inv H0; firstorder; subst; try congruence.
+  * inv H0; firstorder; subst; try congruence.
+  * inv H0.
+    - inv H7. cbn in *. invSome.
+    - rewrite H in H6. now inv H6.
+  * inv H.
+    - inv H6. cbn in *. invSome.
+    - now auto.
+  * inv H0.
+    - inv H7. cbn in *. invSome.
+    - rewrite H in H6. now inv H6.
+  * inv H.
+    - inv H6. cbn in *. invSome.
+    - now auto.
+    - congruence.
+  * inv H.
+    - inv H6. cbn in *. invSome.
+    - now auto.
+    - congruence.
+  * inv H1.
+    - inv H8. cbn in *. invSome.
+    - now auto.
+    - congruence.
+    - congruence.
+  * inv H0. rewrite <-H in H7. now inv H7.
+Qed.
+
+Lemma par_eq : forall T ι (p p' : T) Π Π',
+  ι ↦ p |||| Π = ι ↦ p' |||| Π' -> p = p'.
+Proof.
+  intros. apply equal_f with ι in H as H'.
+  unfold update in H'; break_match_hyp. 
+  2: { apply Nat.eqb_neq in Heqb. congruence. } inversion H'. auto.
+Qed.
+
+Lemma concurrent_determinism :
+  forall Π a ι Π', Π -[a | ι]ₙ-> Π' -> forall Π'', Π -[a | ι]ₙ-> Π'' -> Π' = Π''.
+Proof.
+  intros Π a ι Π' IH. inversion IH; intros; subst.
+  * inv H4.
+    - apply par_eq in H2 as H2'. subst.
+      eapply internal_determinism in H. 2:exact H8. subst. auto. f_equal.
+      extensionality ι''. apply equal_f with ι'' in H2. unfold update in *.
+      break_match_goal; auto.
+    - intuition; try congruence.
+  * inv H5.
+    - apply par_eq in H2 as H2'. inversion H2'. subst.
+      eapply internal_determinism in H0. 2: exact H10. subst.
+      rewrite H in H9. inv H9.
+      f_equal.
+      extensionality ι''. apply equal_f with ι'' in H2. unfold update in *.
+      break_match_goal; auto.
+    - intuition; try congruence.
+  * inv H5.
+    - intuition; try congruence.
+    - intuition; try congruence.
+    - apply par_eq in H2 as H2'. subst.
+      eapply internal_determinism in H. 2: exact H3. subst. f_equal.
+      extensionality ι''. apply equal_f with ι'' in H2. unfold update in *.
+      break_match_goal; auto.
+    - intuition; try congruence.
+    - apply par_eq in H3 as H3'. subst.
+      inv H.
+  * inv H7.
+    - intuition; try congruence.
+    - apply par_eq in H4 as H4'. subst.
+      eapply internal_determinism in H2. 2: exact H14. subst.
+      f_equal. rewrite H in H9. inv H9.
+      rewrite H1 in H13. inv H13.
+      extensionality ι''. apply equal_f with ι'' in H4. unfold update in *.
+      break_match_goal; auto.
+      break_match_goal; auto.
+  * inv H3.
+    - apply par_eq in H0 as H0'. subst.
+      intuition; subst; try congruence. destruct H.
+      inv H1.
+    - unfold update in *. f_equal.
+      extensionality ι'. apply equal_f with ι' in H1. break_match_goal; auto.
+Qed.
+
+Lemma internal_equal :
+  forall p p', inl p -⌈ τ ⌉-> p' -> forall p'' a, inl p -⌈ a ⌉-> p''
+->
+  (a = τ /\ p'' = p') \/
+  (exists t ι ι', a = AArrive ι ι' t
+   /\ exists p''', p' -⌈AArrive ι ι' t⌉-> p''' /\
+   (p'' -⌈ τ ⌉-> p''' \/ p'' = p''')).
+Proof.
+  intros. destruct a.
+  * exfalso. inv H0; inv H; try inv H6; cbn in *; invSome.
+  * right. do 3 eexists. split. reflexivity. inv H0.
+    - inv H.
+      + eexists. split. constructor. left. now constructor.
+      + destruct mb, l0; simpl in *; invSome.
+        eexists. split. constructor.
+        left. now constructor.
+      + eexists. split. constructor.
+        left. destruct mb, l0.
+        ** cbn. unfold mailboxPush. cbn.
+           admit. (* TODO this is wrong, recv_next could not be silent! *)
+        ** admit.
+      + destruct mb, l0; cbn in *; invSome.
+        eexists. split. constructor. left. constructor.
+        cbn. (* TODO: this won't work either (removeMessage + arrive) *)
+        admit.
+      + eexists. split. constructor. left. now constructor.
+      + eexists. split. constructor. left. now constructor.
+      + eexists. split. constructor. left. now constructor.
+    - inv H; admit.
+    - inv H; admit.
+    - inv H; admit.
+    - inv H.
+      all: eexists; split; [constructor|];left; now constructor.
+    - inv H.
+      all: eexists; split; [constructor|];left; now constructor.
+  * exfalso. inv H0; inv H. inv H6; cbn in *; invSome.
+  * exfalso. inv H0; inv H. inv H7; cbn in *; invSome.
+  * left. eapply internal_determinism in H; eauto.
+  * exfalso. inv H0; inv H; inv H6.
+  * exfalso. inv H0; inv H. inv H7. cbn in *. invSome.
+Qed.
+  
+  
+  
+  
+  
+   inv H; inv H0.
+  all: try now inv H2; try destruct mb, l0; cbn in *; invSome.
+  44: {
+  all: try now (inv H2; auto).
+  * eapply step_determinism in H2. 2: exact H9. destruct H2. subst. auto.
+  * right. exists (Message v),source, dest. auto.
+    split; auto. eexists. split. constructor; auto.
+    left. inversion H; subst. now constructor.
+  * right. exists (Exit reason b),source,dest.
+    split; auto. eexists. split. constructor; auto.
+    left. inversion H; subst. now constructor.
+  * right. do 3 eexists. split. reflexivity.
+    intuition; subst; eexists.
+    - split. apply p_exit_terminate. auto. now right.
+    - split. apply p_exit_terminate. right. left. auto. now right.
+    - split. apply p_exit_terminate. right. right. auto. now right.
+  * right. do 3 eexists. split. reflexivity.
+    intuition; subst; eexists.
+    - split. apply p_exit_convert. auto. left. constructor; auto.
+    - split. apply p_exit_convert. auto. left. constructor; auto.
+  * right. do 3 eexists. split. reflexivity.
+    intuition; subst; eexists. split. constructor. do 2 constructor; auto.
+  * right. do 3 eexists. split. reflexivity.
+    intuition; subst; eexists. split. constructor. do 2 constructor; auto.
+  * apply bool_from_lit_val in H9. inversion H2; subst; inversion_is_value.
+Qed.
+
+Theorem internal_is_alive :
+  forall p p', p -⌈AInternal⌉-> p' -> exists pa, p = inl pa.
+Proof.
+  intros. inversion H; subst; try (do 2 eexists; split; reflexivity).
+Qed.
+
+Lemma internal_det :
+  forall n n' n'' ι a, n -[AInternal | ι]ₙ-> n' -> n -[a | ι]ₙ-> n''
+->
+  (a = AInternal /\ n''= n') \/ (exists t ι', a = AArrive ι' ι t /\
+                                 exists n''', n' -[AArrive ι' ι t | ι]ₙ-> n''' /\
+                                 (n'' -[AInternal | ι]ₙ-> n''' \/ n'' = n''')
+                                (* /\
+                                 n'' = modifyMailbox ι ι t n /\
+                                 exists n''', n' -[AArrive t | ι]ₙ-> n''' /\
+                                 n''' = modifyMailbox ι ι t n' *)).
+Proof.
+  intros. inversion H; inversion H0; subst.
+  * inversion H8; subst. apply par_eq in H5. subst.
+    apply internal_is_alive in H1 as H1'. destruct H1'. subst.
+    eapply internal_equal in H7; eauto.
+    destruct H7 as [[? ?] | [? [? [? [? ?]]]]];  congruence.
+  * inversion H9; subst. apply par_eq in H5; subst.
+    eapply internal_is_alive in H1 as H1'. destruct H1'. subst.
+    eapply internal_equal in H8 as H8'. 2: exact H1.
+    destruct H8' as [[? ?] | [? [? [? [? [? ?]]]]]]; try congruence.
+    inversion H3. subst. right.
+    do 2 eexists. split. reflexivity.
+    eexists. split. econstructor; eauto.
+    apply H4.
+    inversion H9. Search update.
+    replace (x2 : p'0 |||| prs) with (x2 : p'0 |||| Π). 2: {
+      extensionality y. unfold update. break_match_goal; auto.
+      apply equal_f with y in H6. unfold update in H6. now rewrite Heqb in H6.
+    }
+    destruct H4 as [_ [? | ?]].
+    - left. now apply n_other.
+    - subst. now right.
+  * inversion H9; subst. apply par_eq in H5; subst.
+    apply internal_is_alive in H1 as H1'. destruct H1'. subst.
+    eapply internal_equal in H7. 2: exact H1. destruct H7 as [[? ?] | [? [? [? [? [? ?]]]]]]; try congruence.
+    - subst. left; split; auto. f_equal. inversion H9.
+      extensionality x'. apply equal_f with x' in H4. unfold update in *. break_match_goal; auto.
+    - subst. inversion H8. 2: destruct H3. 3: destruct H3.
+      3-4: destruct H3. all: try congruence.
+  * inversion H10; subst. apply par_eq in H5. subst.
+    apply internal_is_alive in H1 as H1'. destruct H1'. subst.
+    eapply internal_equal in H9; eauto. destruct H9 as [[? ?] | [? [? [? [? ?]]]]]; congruence.
+  * inversion H7; subst. apply par_eq in H5. subst.
+    inversion H1; subst; try inversion_is_value.
+Qed.
+
+Definition bothSpawn (a1 a2 : Action) : Prop:=
+match a1, a2 with
+| ASpawn _ _ _, ASpawn _ _ _ => True
+| _, _ => False
+end.
+
+Lemma step_chain :
+  forall n n' ι a, n -[a | ι]ₙ-> n' -> forall n'' a' ι' 
+    (Spawns : ~ bothSpawn a a'), n -[a' | ι']ₙ-> n'' ->
+  ι <> ι'
+->
+  exists n''', n' -[a' | ι']ₙ-> n'''.
+Proof.
+  intros n n' ι a IH. inversion IH; intros; subst.
+  * inversion H4; subst.
+    - exists (etherAdd ι'0 ι'1 t0 (etherAdd ι ι' t ether), ι'0 : p'0 |||| ι : p' |||| prs ).
+      replace (ι : p' |||| prs) with (ι'0 : p0 |||| ι : p' |||| prs) at 1.
+      2: { extensionality ι1. unfold update in *. apply equal_f with ι1 in H2.
+           break_match_goal; subst.
+           break_match_goal; subst. eqb_to_eq. congruence. auto.
+           auto.
+         }
+      now constructor.
+    - exists (etherAdd ι ι' t ether'
+              , ι'0 : p'0 |||| ι : p' |||| prs ).
+      replace (ι : p' |||| prs) with (ι'0 : p0 |||| ι : p' |||| prs) at 1.
+      2: { extensionality x. unfold update in *. apply equal_f with x in H1.
+           break_match_goal; subst.
+           break_match_goal; subst. eqb_to_eq. congruence. auto.
+           auto.
+         }
+      constructor. 2: auto.
+      now apply etherPop_greater.
+    - exists (etherAdd ι ι' t ether, ι'0 : p'0 |||| ι : p' |||| prs).
+      replace (ι : p' |||| prs) with (ι'0 : p0 |||| ι : p' |||| prs) at 1.
+      2: { extensionality x. unfold update in *. apply equal_f with x in H1.
+           break_match_goal; subst.
+           break_match_goal; subst. eqb_to_eq. congruence. auto.
+           auto.
+         }
+      now constructor.
+    - exists (etherAdd ι ι' t ether, 
+              ι'1 : inl ([], EApp v1 l, [], [], false) |||| ι'0 : p'0 |||| ι : p' |||| prs).
+      replace (ι : p' |||| prs) with (ι'0 : p0 |||| ι : p' |||| prs) at 1.
+      2: { extensionality x. unfold update in *. apply equal_f with x in H1.
+           break_match_goal; subst.
+           break_match_goal; subst. eqb_to_eq. congruence. auto.
+           auto.
+         }
+      constructor; auto.
+      apply equal_f with ι'1 in H1.
+      unfold update in *. break_match_goal; auto.
+      break_match_goal; subst.
+      + congruence.
+      + now rewrite H1 in H3.
+    - exists (etherAdd ι ι' t ether,
+               ι : p' |||| prs -- ι'0).
+      replace (ι : p' |||| prs) with (ι'0 : inr [] |||| ι : p' |||| prs) at 1.
+      2: { extensionality x. unfold update in *. apply equal_f with x in H2.
+           break_match_goal; subst.
+           break_match_goal; subst. eqb_to_eq. congruence. auto.
+           auto.
+         }
+      rewrite update_swap with (ι := ι); auto.
+      constructor; auto.
+  * inversion H5; subst.
+    - exists (etherAdd ι' ι'0 t0 ether', ι' : p'0 |||| ι : p' |||| prs).
+      replace (ι : p' |||| prs) with (ι' : p0 |||| ι : p' |||| prs) at 1.
+      2: { extensionality x. unfold update in *. apply equal_f with x in H3.
+           break_match_goal; subst.
+           break_match_goal; subst. eqb_to_eq. congruence. auto.
+           auto.
+         }
+      now constructor.
+    - assert (exists ether'', etherPop ι2 ι' ether'  = Some (t0, ether''))
+                                 as [ether'' Eq].
+      {
+         unfold etherPop in H, H3. do 2 break_match_hyp. 1-3: congruence.
+         inversion H. inversion H3. subst.
+         unfold etherPop, update. destruct (ι1 =? ι2) eqn:Eq; eqb_to_eq; subst.
+         * apply Nat.eqb_neq in H6. rewrite H6, Heql. eexists. reflexivity.
+         * rewrite Heql. eexists. reflexivity.
+      }
+      exists (ether''
+              , ι' : p'0 |||| ι : p' |||| prs ).
+      replace (ι : p' |||| prs) with (ι' : p0 |||| ι : p' |||| prs) at 1.
+      2: { extensionality x. unfold update in *. apply equal_f with x in H2.
+           break_match_goal; subst.
+           break_match_goal; subst. eqb_to_eq. congruence. auto.
+           auto.
+         }
+      constructor; auto.
+    - exists (ether', ι' : p'0 |||| ι : p' |||| prs).
+      replace (ι : p' |||| prs) with (ι' : p0 |||| ι : p' |||| prs) at 1.
+      2: { extensionality x. unfold update in *. apply equal_f with x in H2.
+           break_match_goal; subst.
+           break_match_goal; subst. eqb_to_eq. congruence. auto.
+           auto.
+         }
+      now constructor.
+    - exists (ether', 
+              ι'0 : inl ([], EApp v1 l, [], [], false) |||| ι' : p'0 |||| ι : p' |||| prs).
+      replace (ι : p' |||| prs) with (ι' : p0 |||| ι : p' |||| prs) at 1.
+      2: { extensionality x. unfold update in *. apply equal_f with x in H2.
+           break_match_goal; subst.
+           break_match_goal; subst. eqb_to_eq. congruence. auto.
+           auto.
+         }
+      constructor; auto.
+      apply equal_f with ι'0 in H2.
+      unfold update in *. break_match_goal; auto.
+      break_match_goal; subst.
+      + congruence.
+      + now rewrite H2 in H4.
+    - exists (ether',
+               ι : p' |||| prs -- ι').
+      replace (ι : p' |||| prs) with (ι' : inr [] |||| ι : p' |||| prs) at 1.
+      2: { extensionality x. unfold update in *. apply equal_f with x in H3.
+           break_match_goal; subst.
+           break_match_goal; subst. eqb_to_eq. congruence. auto.
+           auto.
+         }
+      rewrite update_swap with (ι := ι); auto.
+      constructor; auto.
+  * inversion H5; subst.
+    - exists (etherAdd ι' ι'0 t ether, ι' : p'0 |||| ι : p' |||| Π).
+      replace (ι : p' |||| Π) with (ι' : p0 |||| ι : p' |||| Π) at 1.
+      2: { extensionality x. unfold update in *. apply equal_f with x in H3.
+           break_match_goal; subst.
+           break_match_goal; subst. eqb_to_eq. congruence. auto.
+           auto.
+         }
+      now constructor.
+    - exists (ether'
+              , ι' : p'0 |||| ι : p' |||| Π ).
+      replace (ι : p' |||| Π) with (ι' : p0 |||| ι : p' |||| Π) at 1.
+      2: { extensionality x. unfold update in *. apply equal_f with x in H2.
+           break_match_goal; subst.
+           break_match_goal; subst. eqb_to_eq. congruence. auto.
+           auto.
+         }
+      constructor; auto.
+    - exists (ether, ι' : p'0 |||| ι : p' |||| Π).
+      replace (ι : p' |||| Π) with (ι' : p0 |||| ι : p' |||| Π) at 1.
+      2: { extensionality x. unfold update in *. apply equal_f with x in H2.
+           break_match_goal; subst.
+           break_match_goal; subst. eqb_to_eq. congruence. auto.
+           auto.
+         }
+      now constructor.
+    - exists (ether, 
+              ι'0 : inl ([], EApp v1 l, [], [], false) |||| ι' : p'0 |||| ι : p' |||| Π).
+      replace (ι : p' |||| Π) with (ι' : p0 |||| ι : p' |||| Π) at 1.
+      2: { extensionality x. unfold update in *. apply equal_f with x in H2.
+           break_match_goal; subst.
+           break_match_goal; subst. eqb_to_eq. congruence. auto.
+           auto.
+         }
+      constructor; auto.
+      apply equal_f with ι'0 in H2.
+      unfold update in *. break_match_goal; auto.
+      break_match_goal; subst.
+      + congruence.
+      + now rewrite H2 in H4.
+    - exists (ether,
+               ι : p' |||| Π -- ι').
+      replace (ι : p' |||| Π) with (ι' : inr [] |||| ι : p' |||| Π) at 1.
+      2: { extensionality ι1. unfold update in *. apply equal_f with ι1 in H3.
+           break_match_goal; subst.
+           break_match_goal; subst. eqb_to_eq. congruence. auto.
+           auto.
+         }
+      rewrite update_swap with (ι := ι); auto.
+      constructor; auto.
+  * inversion H6; subst.
+    - exists (etherAdd ι'0 ι'1 t ether, ι'0 : p'0 |||| 
+                                        ι' : inl ([], EApp v1 l, [], [], false) |||| 
+                                        ι : p' |||| Π).
+      replace (ι' : inl ([], EApp v1 l, [], [], false) |||| ι : p' |||| Π) with 
+              (ι'0 : p0 |||| ι' : inl ([], EApp v1 l, [], [], false) |||| ι : p' |||| Π) at 1.
+      2: { extensionality x. unfold update in *. apply equal_f with x in H4.
+           break_match_goal; subst;
+           break_match_goal; subst; auto.
+           all: break_match_hyp; eqb_to_eq; subst; auto; try congruence.
+           break_match_hyp; congruence.
+         }
+      now constructor.
+    - exists (ether'
+              , ι'0 : p'0 |||| ι' : inl ([], EApp v1 l, [], [], false) 
+                          |||| ι : p' |||| Π ).
+      replace (ι' : inl ([], EApp v1 l, [], [], false) |||| ι : p' |||| Π) with 
+              (ι'0 : p0 |||| ι' : inl ([], EApp v1 l, [], [], false) |||| ι : p' |||| Π) at 1.
+      2: { extensionality x. unfold update in *. apply equal_f with x in H3.
+           break_match_goal; subst;
+           break_match_goal; subst; auto.
+           all: break_match_hyp; eqb_to_eq; subst; auto; try congruence.
+           break_match_hyp; congruence.
+         }
+      constructor; auto.
+    - exists (ether, ι'0 : p'0 |||| ι' : inl ([], EApp v1 l, [], [], false)
+                               |||| ι : p' |||| Π).
+      replace (ι' : inl ([], EApp v1 l, [], [], false) |||| ι : p' |||| Π) with 
+              (ι'0 : p0 |||| ι' : inl ([], EApp v1 l, [], [], false) |||| ι : p' |||| Π) at 1.
+      2: { extensionality x. unfold update in *. apply equal_f with x in H3.
+           break_match_goal; subst;
+           break_match_goal; subst; auto.
+           all: break_match_hyp; eqb_to_eq; subst; auto; try congruence.
+           break_match_hyp; congruence.
+         }
+      now constructor.
+    - (** cannot be sure to generate different spawn PID-s *)
+      exfalso. apply Spawns. cbn. auto.
+    - exists (ether,
+               ι' : inl ([], EApp v1 l, [], [], false) |||| ι : p' |||| Π -- ι'0).
+      replace (ι' : inl ([], EApp v1 l, [], [], false) |||| ι : p' |||| Π) with 
+              (ι'0 : inr [] |||| ι' : inl ([], EApp v1 l, [], [], false) 
+                            |||| ι : p' |||| Π) at 1.
+      2: { extensionality x. unfold update in *. apply equal_f with x in H4.
+           break_match_goal; subst.
+           break_match_goal; subst. eqb_to_eq. subst.
+           break_match_hyp; congruence.
+           break_match_goal; auto. eqb_to_eq. congruence.
+           break_match_goal; auto.
+         }
+      rewrite update_swap with (ι := ι); auto.
+      rewrite update_swap with (ι := ι') (ι' := ι'0); auto.
+      constructor; auto.
+      apply equal_f with ι' in H4. unfold update in H4. cbn in H4.
+      break_match_hyp; eqb_to_eq; auto; subst.
+      break_match_hyp; eqb_to_eq; subst; try congruence; auto.
+      unfold update in H0. break_match_hyp; congruence.
+  * inversion H3; subst.
+    - exists (etherAdd ι' ι'0 t ether, ι' : p' |||| (Π -- ι)).
+      replace (Π -- ι) with (ι' : p |||| (Π -- ι)) at 1.
+      2: { extensionality x. unfold update in *. apply equal_f with x in H1.
+           break_match_goal; subst.
+           break_match_goal; subst. eqb_to_eq. congruence. auto.
+           auto.
+         }
+      now constructor.
+    - exists (ether'
+              , ι' : p' |||| (Π -- ι) ).
+      replace (Π -- ι) with (ι' : p |||| (Π -- ι)) at 1.
+      2: { extensionality x. unfold update in *. apply equal_f with x in H0.
+           break_match_goal; subst.
+           break_match_goal; subst. eqb_to_eq. congruence. auto.
+           auto.
+         }
+      constructor; auto.
+    - exists (ether, ι' : p' |||| (Π -- ι)).
+      replace (Π -- ι) with (ι' : p |||| (Π -- ι)) at 1.
+      2: { extensionality x. unfold update in *. apply equal_f with x in H0.
+           break_match_goal; subst.
+           break_match_goal; subst. eqb_to_eq. congruence. auto.
+           auto.
+         }
+      now constructor.
+    - exists (ether, 
+              ι'0 : inl ([], EApp v1 l, [], [], false) |||| ι' : p' |||| (Π -- ι)).
+      replace (Π -- ι) with (ι' : p |||| (Π -- ι)) at 1.
+      2: { extensionality x. unfold update in *. apply equal_f with x in H0.
+           break_match_goal; subst.
+           break_match_goal; subst. eqb_to_eq. congruence. auto.
+           auto.
+         }
+      constructor; auto.
+      apply equal_f with ι'0 in H0.
+      unfold update in *. break_match_goal; auto.
+      break_match_goal; subst; auto. congruence.
+    - exists (ether, (Π -- ι) -- ι').
+      replace (Π -- ι) with (ι' : inr [] |||| (Π -- ι)) at 1.
+      2: { extensionality x. unfold update in *. apply equal_f with x in H1.
+           break_match_goal; subst. auto.
+           break_match_goal; subst. eqb_to_eq. congruence. auto.
+           break_match_goal; subst; auto.
+         }
+      constructor; auto.
+Qed.
+
+Corollary chain_to_end :
+  forall n n' l, n -[l]ₙ->* n' -> Forall (fun a => a.1 = AInternal) l -> 
+   forall n'' a ι, n -[a | ι]ₙ-> n''
+->
+  (exists n3 n4 l1 l2, a = AInternal /\ 
+    n -[l1]ₙ->* n3 /\ n3 -[a |ι]ₙ-> n4 /\ n4 -[l2]ₙ->* n' /\
+    l = l1 ++ [(a, ι)] ++ l2
+  ) \/ 
+  (exists n''', n' -[a | ι]ₙ-> n''').
+Proof.
+  intros n n' l Steps.
+  dependent induction Steps; intros.
+  * right. eexists. eauto.
+  * inversion H0; subst. simpl in H4. subst.
+    destruct (Nat.eq_dec ι ι0); subst.
+    - eapply internal_det in H1 as H1'. 2: exact H.
+      destruct H1' as [[eq1 eq2] | [t H0']]; subst.
+      + left. exists n, n', [], l. split; auto.
+        split. 2: split. constructor.
+        auto.
+        split; auto.
+      + destruct H0' as [source [eq [n''' [D _]]]]. subst.
+        inversion H1; subst.
+        2: { intuition; try congruence. destruct H4; congruence. }
+        specialize (IHSteps H5 _ _ _ D).
+           destruct IHSteps as [[n3 [n4 [l1 [l2 H2]]]]| [n3 D2]].
+           -- left. destruct H2 as [eq1 [D1 [D2 [ D3 eq2]]]]. subst.
+              congruence.
+           -- right. eexists; eauto.
+    - eapply step_chain in H1. 2: exact H. 2-3: auto.
+      destruct H1. eapply IHSteps in H1 as H1'; auto.
+      destruct H1' as [[n3 [n4 [l1 [l2 H2]]]] | [t H0']]; subst.
+      + left. destruct H2 as [eq1 [D1 [D2 [ D3 eq2]]]]. subst.
+        exists n3, n4, ((AInternal, ι)::l1), l2. split; auto.
+        split. 2: split. 3: split. all: auto.
+        eapply n_trans. 2: exact D1. auto.
+      + right. now exists t.
+Qed.
+
+Lemma internal_keep :
+  forall n n' ι, n -[AInternal | ι]ₙ-> n'
+->
+  forall x, x <> ι -> snd n x = snd n' x.
+Proof.
+  intros. inversion H; subst.
+  simpl. unfold update. break_match_goal; auto. eqb_to_eq. congruence.
+Qed.
+
+(* general case wont work: message ordering is not the same *)
+Theorem diamond_derivations :
+  forall n1 n2 n3 n4 a ι1 ι2, ι1 <> ι2 ->
+  n1 -[AInternal | ι1]ₙ-> n2 -> n1 -[a | ι2]ₙ-> n3 -> n2 -[a | ι2]ₙ-> n4
+->
+  n3 -[AInternal | ι1]ₙ-> n4.
+Proof.
+  intros.
+  inversion H2; subst.
+  * inversion H1; subst.
+    2: { intuition; try congruence. destruct H6; congruence. }
+    inversion H0; subst.
+    assert (p = p0). {
+      apply internal_keep with (x := ι2) in H0. simpl in H0.
+      unfold update in H0. break_match_hyp. now inversion H0. eqb_to_eq. congruence.
+      auto.
+    }
+    subst.
+    subst. eapply internal_determinism in H3. 2: exact H10. subst.
+    assert ((ι1 : p1 |||| ι2 : p' |||| prs0) = ι1 : p1 |||| ι2 : p' |||| prs) as EQ. {
+      extensionality x. unfold update in *. break_match_goal; auto.
+      apply internal_keep with (x := x) in H0. simpl in H0.
+      break_match_goal; auto. eqb_to_eq. auto.
+    }
+    replace (ι2 : p' |||| prs0) with (ι1 : p1 |||| ι2 : p' |||| prs0).
+    replace (ι2 : p' |||| prs) with (ι1 : p'1 |||| ι2 : p' |||| prs).
+    rewrite EQ. constructor; auto.
+    all: unfold update in *; extensionality x; 
+         apply equal_f with x in H5; apply equal_f with x in H12;
+         do 2 break_match_goal; eqb_to_eq; subst; auto; congruence.
+  * inversion H1; subst.
+    inversion H0; subst.
+    2: { intuition; try congruence. destruct H7; congruence. }
+    assert (p = p0). {
+      apply internal_keep with (x := ι2) in H0. simpl in H0.
+      unfold update in H0. break_match_hyp. now inversion H0. eqb_to_eq. congruence.
+      auto.
+    }
+    subst.
+    subst. eapply internal_determinism in H4. 2: exact H12. subst.
+    assert ((ι1 : p1 |||| ι2 : p' |||| prs0) = ι1 : p1 |||| ι2 : p' |||| prs) as EQ. {
+      extensionality x. unfold update in *. break_match_goal; auto.
+      apply internal_keep with (x := x) in H0. simpl in H0.
+      break_match_goal; auto. eqb_to_eq. auto.
+    }
+    replace (ι2 : p' |||| prs0) with (ι1 : p1 |||| ι2 : p' |||| prs0).
+    replace (ι2 : p' |||| prs) with (ι1 : p'1 |||| ι2 : p' |||| prs).
+    rewrite EQ. rewrite H3 in H11. inversion H11. subst. constructor; auto.
+    all: unfold update in *; extensionality x; 
+         apply equal_f with x in H6; apply equal_f with x in H14;
+         do 2 break_match_goal; eqb_to_eq; subst; auto; congruence.
+  * inversion H1; subst.
+    1,2,4,5: intuition; try congruence;
+      match goal with
+      | [H : exists _, _ |- _] => destruct H; congruence
+      | _ => idtac
+      end.
+    - inversion H0; subst.
+      assert (p = inr []). {
+        apply internal_keep with (x := ι2) in H0. simpl in H0.
+        unfold update in H0. break_match_hyp. now inversion H0. eqb_to_eq. congruence.
+        auto.
+      }
+      subst.
+      inversion H3.
+    - inversion H0; subst.
+      assert (p = p0). {
+        apply internal_keep with (x := ι2) in H0. simpl in H0.
+        unfold update in H0. break_match_hyp. now inversion H0. eqb_to_eq. congruence.
+        auto.
+      }
+      subst.
+      subst. eapply internal_determinism in H3. 2: exact H5. subst.
+      assert ((ι1 : p1 |||| ι2 : p' |||| Π0) = ι1 : p1 |||| ι2 : p' |||| Π) as EQ. {
+        extensionality x. unfold update in *. break_match_goal; auto.
+        apply internal_keep with (x := x) in H0. simpl in H0.
+        break_match_goal; auto. eqb_to_eq. auto.
+      }
+      replace (ι2 : p' |||| Π0) with (ι1 : p1 |||| ι2 : p' |||| Π0).
+      replace (ι2 : p' |||| Π) with (ι1 : p'1 |||| ι2 : p' |||| Π).
+      rewrite EQ. constructor; auto.
+      1-2: unfold update in *; extensionality x; 
+           apply equal_f with x in H8; apply equal_f with x in H13;
+           do 2 break_match_goal; eqb_to_eq; subst; auto; congruence.
+  * inversion H1; subst.
+    1: intuition; try congruence; destruct H8; congruence.
+    inversion H0; subst.
+    assert (p = p0). {
+      apply internal_keep with (x := ι2) in H0. simpl in H0.
+      unfold update in H0. break_match_hyp. now inversion H0. eqb_to_eq. congruence.
+      auto.
+    }
+    subst.
+    subst. eapply internal_determinism in H5. 2: exact H14. subst.
+    assert ((ι1 : p1 |||| ι' : inl ([], EApp v1 l0, [], [], false) |||| ι2 : p' |||| Π0) = 
+             ι1 : p1 |||| ι' : inl ([], EApp v1 l0, [], [], false) |||| ι2 : p' |||| Π) as EQ. {
+      extensionality x. unfold update in *. break_match_goal; auto.
+      break_match_goal; auto.
+      apply internal_keep with (x := x) in H0. simpl in H0.
+      break_match_goal; auto.
+      eqb_to_eq. auto.
+    }
+    rewrite H3 in H10. inversion H10. subst.
+    replace (ι' : inl ([], EApp v1 l0, [], [], false) |||| ι2 : p' |||| Π0) with
+            (ι1 : p1 |||| ι' : inl ([], EApp v1 l0, [], [], false) |||| ι2 : p' |||| Π0).
+    replace (ι' : inl ([], EApp v1 l0, [], [], false) |||| ι2 : p' |||| Π) with
+            (ι1 : p'1 |||| ι' : inl ([], EApp v1 l0, [], [], false) |||| ι2 : p' |||| Π).
+    rewrite EQ. apply n_other; auto.
+    clear EQ H1 H2 H0.
+    all: unfold update in *; extensionality x;
+         apply equal_f with x in H7; apply equal_f with x in H15;
+         do 2 break_match_goal; eqb_to_eq; subst; auto; try congruence.
+    - break_match_goal; eqb_to_eq; auto. subst. congruence.
+    - break_match_goal; eqb_to_eq; auto. subst. congruence.
+  * inversion H1; subst.
+    1: intuition; try congruence. destruct H5; congruence.
+    - inversion H0; subst.
+      assert (p = inr []). {
+        apply internal_keep with (x := ι2) in H0. simpl in H0.
+        unfold update in H0. break_match_hyp. now inversion H0. eqb_to_eq. congruence.
+        auto.
+      }
+      subst.
+      inversion H3.
+    - inversion H0. subst.
+      assert ((ι1 : p |||| (Π0 -- ι2)) = 
+               ι1 : p |||| (Π  -- ι2)) as EQ. {
+        extensionality x. unfold update in *. break_match_goal; auto.
+        apply internal_keep with (x := x) in H0. simpl in H0.
+        break_match_goal; auto. eqb_to_eq. auto.
+      }
+      replace (Π0 -- ι2) with
+              (ι1 : p |||| (Π0 -- ι2)).
+      replace (Π -- ι2) with
+              (ι1 : p' |||| (Π -- ι2)).
+      rewrite EQ. constructor; auto.
+      all: unfold update in *; extensionality x;
+       apply equal_f with x in H4; apply equal_f with x in H9;
+       do 2 break_match_goal; eqb_to_eq; subst; auto; try congruence.
+Qed.
+
+Theorem delay_internal_same :
+  forall n n1 ι,   n -[AInternal | ι]ₙ-> n1 ->
+  forall n2 a, n1 -[a | ι]ₙ-> n2 ->
+       forall n3, n -[a | ι]ₙ-> n3
+->
+  n3 -[AInternal | ι]ₙ-> n2 \/ n3 = n2.
+Proof.
+  intros. inversion H; subst.
+  eapply internal_det in H1 as H1'. 2: exact H.
+  destruct H1' as [[eq1 eq2]| [t [? [eq [n'' D]]]]]; subst.
+  * auto.
+  * inversion H0; subst.
+    2: { intuition; try congruence; destruct H3; congruence. }
+    simpl. apply par_eq in H5 as H5'. subst.
+    inversion H1; subst.
+    - simpl. apply par_eq in H6 as H5'. subst.
+      clear H9 H7 H3.
+      replace (ι : p'1 |||| prs0) with (ι : p'1 |||| prs).
+      2: { extensionality xx.
+           apply equal_f with xx in H5. apply equal_f with xx in H6.
+           unfold update in *. break_match_hyp; auto. now rewrite <- H5 in H6.
+         }
+      rewrite H11 in H15. inversion H15. subst.
+      inversion H12; subst.
+      + left. apply n_other.
+        inversion H16; subst.
+        ** inversion H2; subst. now constructor.
+        ** auto.
+      (* drop signal *)
+      + intuition. subst.
+        all: inversion H16; subst; intuition; subst; try congruence.
+        ** left. constructor. inversion H2; subst. now constructor. auto.
+        ** left. constructor. inversion H2; subst. auto. auto.
+        ** left. constructor. inversion H2; subst. auto.
+        ** left. constructor. inversion H2; subst. auto.
+        ** left. constructor. inversion H2; subst. now constructor. auto.
+        ** left. constructor. inversion H2; subst. auto. auto.
+        ** inversion H2.
+        ** inversion H2.
+        ** inversion H2; subst. left. now do 2 constructor.
+        ** inversion H2; subst. left. now do 2 constructor.
+        ** inversion H2; subst. left. congruence.
+        ** inversion H2; subst. left. congruence.
+        ** inversion H2; subst. left. now do 2 constructor.
+        ** inversion H2; subst. left. now do 2 constructor.
+        ** inversion H2; subst. left. congruence.
+        ** inversion H2; subst. left. congruence.
+      (* terminate process *)
+      + inversion H2; subst. inversion H16; subst; intuition; subst; try congruence.
+        all: now right.
+      (* add signal to message queue *)
+      + intuition. subst.
+        all: inversion H16; subst; intuition; subst; try congruence.
+        all: left; constructor; inversion H2; subst; auto.
+        ** constructor; auto.
+        ** constructor; auto.
+        ** congruence.
+        ** constructor; auto.
+        ** congruence.
+        ** constructor; auto.
+      + left. apply n_other.
+        inversion H16; subst.
+        ** inversion H2; subst. now constructor.
+        ** auto.
+      + left. apply n_other.
+        inversion H16; subst.
+        ** inversion H2; subst. now constructor.
+        ** auto.
+    - intuition; subst; try congruence. now inversion H3.
+      now inversion H3.
+      now inversion H3.
+      now inversion H3.
+Qed.
+
+Corollary chain_to_front_iff :
+  forall n n', n -->* n' -> forall a ι n'' n3, (* a <> AInternal -> *)
+  n' -[a | ι]ₙ-> n'' ->
+  n  -[a | ι]ₙ-> n3
+->
+  n3 -->* n''.
+Proof.
+  intros n n' D.
+  destruct D as [l [All D]]. induction D; intros.
+  * eapply concurrent_determinism in H. 2: exact H0. subst. apply internals_refl.
+  * inversion All; simpl in H4. subst.
+    destruct (Nat.eq_dec ι0 ι).
+    - subst.
+      eapply internal_det in H1 as H2'. 2: exact H.
+      destruct H2' as [[? ?] | [t [ι' [? [n4 [D1 _]]]]]]; subst.
+      + eapply internals_trans.
+        exists l. split; eauto.
+        exists [(AInternal, ι)]. split. repeat constructor.
+        eapply n_trans; eauto. constructor.
+      + epose proof (delay_internal_same _ _ _ H _ _ D1 _ H1).
+        epose proof (IHD H5 _ _ _ _ H0 D1).
+        eapply internals_trans. 2: exact H3.
+        destruct H2.
+        ** exists [(AInternal, ι)]. split. repeat constructor.
+           eapply n_trans. exact H2. apply n_refl.
+        ** subst. apply internals_refl.
+    - apply not_eq_sym in n0.
+      epose proof (D2 := step_chain _ _ _ _ H _ _ _ _ H1 n0).
+      destruct D2 as [n4 D2].
+      epose proof (IHD H5 _ _ _ _ H0 D2).
+
+      eapply internals_trans. 2: exact H2.
+      exists [(AInternal, ι)]. split. repeat constructor.
+      eapply n_trans. 2: apply n_refl.
+      clear IHD H5 D All H2 H0.
+      now epose proof (diamond_derivations _ _ _ _ _ _ _ n0 H H1 D2).
+  Unshelve.
+  ** intro. destruct a0; auto.
+Qed.
+
+Theorem split_reduction :
+  forall l1 l2 Π Π'', Π -[l1 ++ l2]ₙ->* Π'' ->
+   exists Π', Π -[l1]ₙ->* Π' /\
+                    Π' -[l2]ₙ->* Π''.
+Proof.
+  intros. dependent induction H.
+  * exists n. intuition; destruct l1, l2; inversion x; constructor.
+  * destruct l1; simpl in *.
+    - destruct l2; inversion x; subst; clear x.
+      specialize (IHclosureNodeSem [] l2 eq_refl).
+      destruct IHclosureNodeSem as [Π' [D1 D2]].
+      exists n. intuition. constructor.
+      econstructor.
+      + inversion D1; subst. exact H.
+      + auto.
+    - inversion x; subst; clear x.
+      specialize (IHclosureNodeSem l1 l2 eq_refl).
+      destruct IHclosureNodeSem as [Π' [D1 D2]].
+      exists Π'. intuition. econstructor. exact H. auto.
+Qed.
+
+Lemma no_ether_pop : forall l Π Π',
+  Π -[ l ]ₙ->* Π' ->
+  forall ι ι' sigs s sigs',
+  ~In (AArrive ι ι' s, ι') l ->
+  fst Π ι ι' = sigs ++ s :: sigs' ->
+  exists sigs1 sigs2, fst Π' ι ι' = sigs1 ++ s :: sigs' ++ sigs2 /\ 
+                      exists sigs1_1, sigs = sigs1_1 ++ sigs1.
+Proof.
+  intros ? ? ? D. induction D; intros.
+  * eexists. exists []. rewrite app_nil_r. split. exact H0.
+    exists []. reflexivity.
+  * apply not_in_cons in H0 as [H0_1 H0_2].
+    inversion H; subst.
+    (* Send: potentially puts something at the end *)
+    - unfold etherAdd, update in IHD. cbn in IHD.
+      destruct (ι =? ι0) eqn:Eq1. destruct (ι'0 =? ι') eqn:Eq2.
+      + eqb_to_eq; subst.
+        specialize (IHD ι0 ι' sigs s (sigs' ++ [t]) H0_2).
+        cbn in *. rewrite H1 in IHD. rewrite <- app_assoc in IHD.
+        assert (sigs ++ (s :: sigs') ++ [t] = sigs ++ s :: sigs' ++ [t]). {
+          f_equal.
+        }
+        do 2 rewrite Nat.eqb_refl in IHD.
+        apply IHD in H2 as [sigs1 [sigs2 [IHD' IHD'']]].
+        rewrite IHD'. exists sigs1. exists ([t] ++ sigs2).
+        do 2 f_equal. now rewrite app_assoc.
+      + cbn in H1.
+        specialize (IHD ι0 ι' sigs s sigs' H0_2).
+        rewrite Eq1, Eq2 in IHD.
+        eqb_to_eq. subst. rewrite H1 in IHD. apply IHD. reflexivity.
+      + cbn in H1.
+        specialize (IHD ι0 ι' sigs s sigs' H0_2).
+        rewrite Eq1, H1 in IHD. apply IHD. reflexivity.
+    (* Arrive: potentially removes something *)
+    - cbn in *.
+      destruct (ι0 =? ι2) eqn:Eq1.
+      + destruct (ι' =? ι) eqn:Eq2.
+        ** eqb_to_eq. subst.
+           destruct sigs.
+           -- unfold etherPop in H0. rewrite H1 in H0. cbn in H0. inversion H0.
+              congruence.
+           -- unfold etherPop in H0. break_match_hyp. congruence.
+              inversion H0. inversion H1. subst. clear H0 H1.
+              specialize (IHD ι2 ι sigs s sigs' H0_2).
+              unfold update in IHD. do 2 rewrite Nat.eqb_refl in IHD.
+              specialize (IHD eq_refl).
+              destruct IHD as [sigs1 [sigs2 [Eq1 [sigs1_1 Eq2]]]].
+              subst. do 2 eexists. split. eauto. exists (s0 :: sigs1_1).
+              simpl. reflexivity.
+        ** unfold etherPop in H0. break_match_hyp. congruence.
+           inversion H0. subst. eapply IHD in H0_2. apply H0_2.
+           unfold update. rewrite Nat.eqb_sym in Eq1. rewrite Eq1.
+           rewrite Nat.eqb_sym in Eq2. rewrite Eq2. eqb_to_eq. subst. eauto.
+      + unfold etherPop in H0. break_match_hyp. congruence.
+        inversion H0. subst. eapply IHD in H0_2. apply H0_2.
+        unfold update. rewrite Nat.eqb_sym in Eq1. rewrite Eq1. eauto.
+    (* Other actions do not modify the ether *)
+    - eapply IHD. auto. cbn in *. rewrite H1. reflexivity.
+    - eapply IHD. auto. cbn in *. rewrite H1. reflexivity.
+    - eapply IHD. auto. cbn in *. rewrite H1. reflexivity.
+Qed.
+
+
+(** Signal ordering tests: *)
+Lemma signal_ordering :
+  forall l Π (ι ι' : PID) s1 s2 Π' Π'' Π''' (NEQ : s1 <> s2),
+            Π -[ASend ι ι' s1 | ι]ₙ-> Π' ->
+            Π' -[ASend ι ι' s2 | ι]ₙ-> Π'' ->
+            ~In (AArrive ι ι' s1, ι') l ->
+            ~In s1 (fst Π ι ι') ->
+            ~In s2 (fst Π ι ι') ->
+            Π'' -[l]ₙ->* Π''' ->
+            ~exists Σ, Π''' -[AArrive ι ι' s2 | ι']ₙ-> Σ.
+Proof.
+  intros. inversion H. inversion H0. subst.
+  2-3: intuition; try congruence.
+  2: inversion H19; congruence.
+  2: inversion H12; congruence.
+  cbn in *. clear H14 H7 H0 H H11 H18.
+  inversion H13; subst. clear H13.
+  assert (exists sigs sigs', etherAdd ι ι' s2 (etherAdd ι ι' s1 ether) ι ι' = sigs ++ s1 :: sigs') as [sigs1 [sigs2 H]]. {
+    unfold etherAdd, update. do 2 rewrite Nat.eqb_refl.
+    exists (ether ι ι'), [s2]. now rewrite <- app_assoc.
+  }
+  epose proof (no_ether_pop l _ _ H4 _ _ _ _ _ H1 H).
+  intro. destruct H6 as [Π''''].
+  destruct H0 as [sigs11 [sigs3]].
+  clear H1 H4. inversion H6; subst.
+  2: { intuition; try congruence. destruct H0; congruence. }
+  clear H8. destruct H0 as [H0 H0_1].
+  cbn in *. unfold etherPop, update in H11. rewrite H0 in H11.
+  destruct sigs11; cbn in *. inversion H11. congruence.
+  cbn in *. inversion H11; subst. clear H6 H11.
+  unfold etherAdd, update in H. do 2 rewrite Nat.eqb_refl in H.
+  rewrite <- app_assoc in H.
+  destruct H0_1. subst.
+  simpl in H.
+  rewrite <- app_assoc in H.
+  now apply in_list_order in H.
 Qed.
 
