src/Concurrent/NodeSemantics.v
@@ -148,7 +148,7 @@ Inductive nodeSemantics : Node -> Action -> PID -> Node -> Prop :=
 (** internal actions *)
 | n_other p p' a Π (ι : PID) ether:
   p -⌈a⌉-> p' ->
-  (a = τ \/ a = ASelf ι \/ (exists t, a = AReceive t) \/ a = ATerminate \/ a = ASetFlag)
+  (a = τ \/ a = ASelf ι \/ a = ATerminate \/ a = ASetFlag)
 ->
    (ether, ι ↦ p |||| Π) -[a| ι]ₙ-> (ether, ι ↦ p' |||| Π)
 
